

# CS 2LC3

## Logical Reasoning for Computer Science

---

# Tutorial 2

Mahdee Jodayree

Habib Ben Abdallah

McMaster University

September 23, 2022

# Outline

---

- ❖ Announcements / Reminders
- ❖ Syntax and evaluation of Boolean expressions
- ❖ Satisfiability, validity, and duality
- ❖ Modeling English propositions
- ❖ Equivalence and true
- ❖ Negation, inequivalence and false
- ❖ Disjunction
- ❖ Conjunction

# Announcements

---

- ❖ Assignment 1 is posted on the course website and it is due on October 3 (Monday), 2022, 23:59 via Avenue.
- ❖ The submission avenue option is already activated on the avenue.

**Instructions: For all assignments, the students must submit their solutions to**

**Avenue → Assessments → Assignment #**

**Students can solve the exercises on paper, use a smartphone app called [CamScanner](#), convert their entire solution into a single PDF file, and submit it to Avenue.**

**You can also use an iPad or any other software to write your assignment and as long as you convert it into a readable PDF file.**

**The maximum upload file size is 2 GB in Avenue for each submission.**

**Please make sure that the final PDF file is readable.**

**Students, who wish to use Microsoft word and do not have Microsoft Word on their computer, are suggested to use google document editor ([Google Docs](#)). This online software allows you to convert your final file into a PDF file.**

**There will be a mark deduction for not following the submission instruction.**

**Please first finish the assignment on your local computer and, at the end, and attach your solution as a PDF file.**

**You will have an unlimited number of submissions until the deadline.**

Before we can answer exercise 2.1, we need to understand the following operators from the textbook.

Operator  $=$  is *conventional equality*

Operator  $\equiv$  is **equivalence** (second name of  $=$  )

Operator  $\neq$  is *conventional inequality*

Operator  $\nabla$  is **inequivalence** or *xor*

Operator  $\vee$  is called *disjunction* or *or*

Operator  $\wedge$  is called *conjunction* or *and*

Operator  $\Rightarrow$  is called *implication*

Operator  $\Leftarrow$  is called *consequence* or *antecedent*

Page 27 of textbook fully explains the above operator, lets review page 27 of the textbook.

|                   |            |                   |
|-------------------|------------|-------------------|
| $b = c$           | is read as | “b equals c”      |
| $b \equiv c$      | is read as | “b equivaless c”  |
| $b \neq c$        | is read as | “b differ from c” |
| $b \ncong c$      | is read as | “b differ from c” |
| $b \vee c$        | is read as | “b or c”          |
| $b \wedge c$      | is read as | “b and c”         |
| $b \Rightarrow c$ | is read as | “b implies c”     |
| $b \Leftarrow c$  | is read as | “c follows b”     |

Page 27 of textbook

If we were given  $n = \text{false}$  and  $p = \text{true}$ , what is the value of the final expression?

$$(n \Rightarrow p)$$

Before we can answer exercise 2.1, we need to understand the following table from the textbook.

$(n \Rightarrow p)$  is true

$n = f$  and  $p = t$

|     |     | $\vee$ | $\Leftarrow$ | $\Rightarrow$ | $=$ | $\wedge$ | $\neq$ | $\neq$ | $\neq$ | $\neq$ | $\neq$ | $\neq$ | $\neq$ | $\neq$ | $\neq$ | $\neq$ | $\neq$ | $\neq$ |
|-----|-----|--------|--------------|---------------|-----|----------|--------|--------|--------|--------|--------|--------|--------|--------|--------|--------|--------|--------|
| $t$ | $t$ | $t$    | $t$          | $t$           | $t$ | $t$      | $t$    | $t$    | $t$    | $f$    | $f$    | $f$    | $f$    | $f$    | $f$    | $f$    | $f$    | $f$    |
| $t$ | $f$ | $t$    | $t$          | $t$           | $f$ | $f$      | $f$    | $f$    | $f$    | $t$    | $t$    | $t$    | $t$    | $f$    | $f$    | $f$    | $f$    | $f$    |
| $f$ | $t$ | $t$    | $t$          | $f$           | $f$ | $t$      | $f$    | $f$    | $f$    | $t$    | $t$    | $f$    | $f$    | $t$    | $t$    | $f$    | $f$    | $f$    |
| $f$ | $f$ | $t$    | $f$          | $t$           | $f$ | $t$      | $f$    | $t$    | $f$    | $t$    | $f$    | $t$    | $f$    | $t$    | $f$    | $t$    | $f$    | $f$    |

Note: *true* is abbreviated by *t* and *false* by *f*

The above table is from Chapter 2, page 26 of textbook.



Given

$m$ : *false*

$n$ : *true*

What does the following evaluates to?

$$m \equiv n$$

$$m \equiv n$$

If m: false

n: true

$m \equiv n$  is false

If m: false

n: false

$m \equiv n$  is true

# Syntax and evaluation of Boolean expressions

---

**2.1** Each line below contains an expression and two states  $S0$  and  $S1$  (using  $t$  for *true* and  $f$  for *false*). Evaluate the expression in both states.

| expression |   | state $S0$ |     |     |     | state $S1$ |     |     |     |
|------------|---|------------|-----|-----|-----|------------|-----|-----|-----|
|            |   | $m$        | $n$ | $p$ | $q$ | $m$        | $n$ | $p$ | $q$ |
| (f)        | $m \vee (n \Rightarrow p)$              | $t$        | $f$ | $t$ | $t$ | $t$        | $t$ | $f$ | $t$ |
| (j)        | $(m \equiv n) \wedge (p \Rightarrow q)$ | $f$        | $t$ | $f$ | $t$ | $t$        | $t$ | $f$ | $f$ |

# Syntax and evaluation of Boolean expressions

---

**2.1** Each line below contains an expression and two states  $S0$  and  $S1$  (using  $t$  for *true* and  $f$  for *false*). Evaluate the expression in both states.

| expression                     | state $S0$ |     |     |     | state $S1$ |     |     |     |
|--------------------------------|------------|-----|-----|-----|------------|-----|-----|-----|
|                                | $m$        | $n$ | $p$ | $q$ | $m$        | $n$ | $p$ | $q$ |
| (f) $m \vee (n \Rightarrow p)$ | $t$        | $f$ | $t$ | $t$ | $t$        | $t$ | $f$ | $t$ |

In  $S0$ ,  $m \vee (n \Rightarrow p)$  evaluates to  $t \vee (f \Rightarrow t)$ .

$(f \Rightarrow t) \equiv t$  and  $t \vee t \equiv t$ , therefore  $t \vee (f \Rightarrow t) \equiv t$ .

In  $S1$ ,  $m \vee (n \Rightarrow p)$  evaluates to  $t \vee (t \Rightarrow f)$ .

$(t \Rightarrow f) \equiv f$  and  $t \vee f \equiv t$ , therefore  $t \vee (t \Rightarrow f) \equiv t$ .

# Syntax and evaluation of Boolean expressions

---

**2.1** Each line below contains an expression and two states  $S0$  and  $S1$  (using  $t$  for *true* and  $f$  for *false*). Evaluate the expression in both states.

| expression                                  | state $S0$ |     |     |     | state $S1$ |     |     |     |
|---|------------|-----|-----|-----|------------|-----|-----|-----|
|   | $m$        | $n$ | $p$ | $q$ | $m$        | $n$ | $p$ | $q$ |
| (j) $(m \equiv n) \wedge (p \Rightarrow q)$ | $f$        | $t$ | $f$ | $t$ | $t$        | $t$ | $f$ | $f$ |

In  $S0$ ,  $(m \equiv n) \wedge (p \Rightarrow q)$  evaluates to  $(f \equiv t) \wedge (f \Rightarrow t)$ .



$(f \equiv t) \equiv f$ ,  $(f \Rightarrow t) \equiv t$ , and  $f \wedge t \equiv f$  therefore  $(f \equiv t) \wedge (f \Rightarrow t) \equiv f$ .

In  $S1$ ,  $(m \equiv n) \wedge (p \Rightarrow q)$  evaluates to  $(t \equiv t) \wedge (f \Rightarrow f)$ .

$(t \equiv t) \equiv t$ ,  $(f \Rightarrow f) \equiv t$ , and  $t \wedge t \equiv t$  therefore  $(t \equiv t) \wedge (f \Rightarrow f) \equiv t$ .

# What if there was no parentheses?

Each line below contains an expression and two states  $S0$  and  $S1$  (using  $t$  for *true* and  $f$  for *false*). Evaluate the expression in both states.

| expression   | state $S0$ |     |     |     | state $S1$ |     |     |     |
|--|------------|-----|-----|-----|------------|-----|-----|-----|
|  | $m$        | $n$ | $p$ | $q$ | $m$        | $n$ | $p$ | $q$ |
|  $m \equiv n \wedge p \Rightarrow q$  | $f$        | $t$ | $f$ | $t$ | $t$        | $t$ | $f$ | $f$ |

To answer this question we must understand the table of precedence on page 2 of the textbook.

### Table of Precedences

- (a)  $[x := e]$  (textual substitution) (highest precedence)
- (b)  $.$  (function application)
- (c) unary prefix operators:  $+ \ - \ \neg \ \# \ \sim \ \mathcal{P}$
- (d)  $**$
- (e)  $\cdot \ / \ \div \ \mathbf{mod} \ \mathbf{gcd}$
- (f)  $+ \ - \ \cup \ \cap \ \times \ \circ \ \bullet$
- (g)  $\downarrow \ \uparrow$
- (h)  $\#$
- (i)  $\triangleleft \ \triangleright \ \wedge$
- (j)  $= \ < \ > \ \in \ \subset \ \subseteq \ \supset \ \supseteq \ |$  (conjunctive, see page 29)
- (k)  $\vee \ \wedge$
- (l)  $\Rightarrow \ \Leftarrow$
- (m)  $\equiv$  (lowest precedence)

All nonassociative binary infix operators associate to the left, except  $**$ ,  $\triangleleft$ , and  $\Rightarrow$ , which associate to the right.

The operators on lines (j), (l), and (m) may have a slash  $/$  through them to denote negation —e.g.  $b \neq c$  is an abbreviation for  $\neg(b \equiv c)$ .

From page 2 of textbook.

# Syntax and evaluation of Boolean expressions

---

**2.2** Write truth tables to compute values for the following expressions in all states.

(e)  $\neg b \Rightarrow (b \vee c)$

(f)  $\neg b \equiv (b \vee c)$



# Syntax and evaluation of Boolean expressions

---

**2.2** Write truth tables to compute values for the following expressions in all states.

(e)  $\neg b \Rightarrow (b \vee c)$

| $b$ | $c$ | $\neg b$ | $b \vee c$ | $\neg b \Rightarrow (b \vee c)$ |
|-----|-----|----------|------------|---------------------------------|
| $t$ | $t$ | $f$      | $t$        | $t$                             |
| $t$ | $f$ | $f$      | $t$        | $t$                             |
| $f$ | $t$ | $t$      | $t$        | $t$                             |
| $f$ | $f$ | $t$      | $f$        | $f$                             |

# Syntax and evaluation of Boolean expressions

---

**2.2** Write truth tables to compute values for the following expressions in all states.

(f)  $\neg b \equiv (b \vee c)$

| $b$ | $c$ | $\neg b$ | $b \vee c$ | $\neg b \equiv (b \vee c)$ |
|-----|-----|----------|------------|----------------------------|
| $t$ | $t$ | $f$      | $t$        | $f$                        |
| $t$ | $f$ | $f$      | $t$        | $f$                        |
| $f$ | $t$ | $t$      | $t$        | $t$                        |
| $f$ | $f$ | $t$      | $f$        | $f$                        |

# Satisfiability, validity, and duality

---

**2.3** Write the duals  $P_D$  for each of the following expressions  $P$ .

(e)  $\neg false \Rightarrow b \vee c$

(h)  $(b \equiv c) \equiv (b \Rightarrow c) \wedge (c \Rightarrow b)$

**(2.2) Definition.** The *dual*  $P_D$  of a boolean expression  $P$  is constructed from  $P$  by interchanging occurrences of

*true* and *false*,  
 $\wedge$  and  $\vee$ ,  
 $\equiv$  and  $\neq$ ,  
 $\Rightarrow$  and  $\nRightarrow$ , and  
 $\Leftarrow$  and  $\nLeftarrow$ .

# Satisfiability, validity, and duality

---

**2.3** Write the duals  $P_D$  for each of the following expressions  $P$ .

(e)  $\neg \text{false} \Rightarrow b \vee c$

$\neg \text{true} \not\equiv b \wedge c$

# Satisfiability, validity, and duality

---

**2.3** Write the duals  $P_D$  for each of the following expressions  $P$ .

(h)  $(b \equiv c) \equiv (b \Rightarrow c) \wedge (c \Rightarrow b)$   
 $(b \not\equiv c) \not\equiv (b \not\Rightarrow c) \vee (c \not\Rightarrow b)$

# Satisfiability, validity, and duality

---

**2.4** For each expression  $P \equiv Q$  below, write the expression  $P_D \equiv Q_D$ .

(g)  $p \wedge (q \vee r) \equiv (p \wedge q) \vee (p \wedge r)$

(h)  $p \equiv q \equiv q \equiv p$

# Satisfiability, validity, and duality

---

**2.4** For each expression  $P \equiv Q$  below, write the expression  $P_D \equiv Q_D$ .

$$(g) \quad p \wedge (q \vee r) \equiv (p \wedge q) \vee (p \wedge r)$$

$$(g) \quad p \vee (q \wedge r) \equiv (p \vee q) \wedge (p \vee r)$$

$$(h) \quad p \equiv q \equiv q \equiv p$$

$$P_D \quad (h) \quad p \not\equiv q \equiv q \not\equiv p \quad Q_D$$

$$\text{or } \boxed{p} \equiv \boxed{q \not\equiv q \not\equiv p}$$

$$\text{or } p \not\equiv q \not\equiv q \equiv p$$

$$P_D \quad (h) \quad p \not\equiv q \equiv q \not\equiv p$$

$$\text{or } p \equiv q \not\equiv q \not\equiv p$$

$$\text{or } \boxed{p \not\equiv q \not\equiv q} \equiv \boxed{p} \quad Q_D$$

$$P_D \quad (h) \quad \boxed{p \not\equiv q} \equiv \boxed{q \not\equiv p} \quad Q_D$$

$$\text{or } p \equiv q \not\equiv q \not\equiv p$$

$$\text{or } p \not\equiv q \not\equiv q \equiv p$$



# Satisfiability, validity, and duality

---

**2.4** For each expression  $P \equiv Q$  below, write the expression  $P_D \equiv Q_D$ .

(h)  $p \equiv q \equiv q \equiv p$

(h)  $p \not\equiv q \equiv q \not\equiv p$

or  $p \equiv q \not\equiv q \not\equiv p$

or  $p \not\equiv q \not\equiv q \equiv p$

Lets assume

$p : \text{true}$

$q : \text{true}$

# Modeling English propositions

---

**2.5** Translate the following English statements into boolean expressions.

- (a) Whether or not it's raining, I'm going swimming.
- (f) If it rains cats and dogs while I am going swimming, I'll eat my hat.

# Modeling English propositions

---

**2.5** Translate the following English statements into boolean expressions.

(a) Whether or not it's raining, I'm going swimming.

(f) If it rains cats and dogs while I am going swimming, I'll eat my hat.

Associate identifiers with the primitive subexpressions as follows.

$r$  : It's raining

$sd$  : It's raining dogs

$s$  : I'm going swimming

$eh$  : I'll eat my hat

$sc$  : It's raining cats

# Modeling English propositions

---

**2.5** Translate the following English statements into boolean expressions.

(a) Whether or not it's raining, I'm going swimming.

(f) If it rains cats and dogs while I am going swimming, I'll eat my hat.

Associate identifiers with the primitive subexpressions as follows.

$r$  : It's raining

$sd$  : It's raining dogs

$s$  : I'm going swimming

$eh$  : I'll eat my hat

$sc$  : It's raining cats

The translations are then

$$(a) \quad r \vee \neg r \Rightarrow s$$

$$(f) \quad sc \wedge sd \wedge s \Rightarrow eh$$

# Modeling English propositions

---

**2.6** Translate the following English statements into boolean expressions.

- (b) Exactly one of  $p$  and  $q$  is *true*.
- (c) Zero, two, or four of  $p$ ,  $q$ ,  $r$ , and  $s$  are *true*.

# Modeling English propositions

---

**2.6** Translate the following English statements into boolean expressions.

(b) Exactly one of  $p$  and  $q$  is *true* .

(b)  $\neg(p \equiv q)$  , or  $p \not\equiv q$

$$\neg p \equiv q$$

$$p \not\equiv q \longleftarrow (p \wedge \neg q) \vee (\neg p \wedge q) \equiv p \not\equiv q$$

# Modeling English propositions

**2.6** Translate the following English statements into boolean expressions.

(c) Zero, two, or four of  $p$ ,  $q$ ,  $r$ , and  $s$  are *true*.

$$p \equiv q \equiv r \equiv s$$

**Solution 3:**

Or we can answer it the following way

**Solution 2:** Or we can answer it the following way

$$\begin{aligned} &(\neg p \wedge \neg q \wedge \neg r \wedge \neg s) \\ &\vee \\ &(p \wedge q \wedge \neg r \wedge \neg s) \\ &\vee \\ &(p \wedge r \wedge \neg q \wedge \neg s) \end{aligned}$$

| $p$ | $q$ | $r$ | $s$ | $P \equiv q \equiv r \equiv s$ |
|-----|-----|-----|-----|--------------------------------|
| F   | F   | F   | F   | T                              |
| F   | F   | F   | T   | F                              |
| F   | F   | T   | F   | F                              |
| F   | F   | T   | T   | T                              |
| F   | T   | F   | F   | F                              |
| F   | T   | F   | T   | T                              |

we can determine without any additional formal manipulation that

$false = false = false = true$  is false,

because three (an odd number) of its equivalents are false



# Modeling English propositions

**2.8** Translate the following English statement into a boolean expression.  $v$  is in  $b[1..10]$  means that if  $v$  is in  $b[11..20]$  then it is not in  $b[11..20]$ .

**TABLE 2.3.** TRANSLATION OF ENGLISH WORDS

|                         |         |                   |
|-------------------------|---------|-------------------|
| and, but                | becomes | $\wedge$          |
| or                      | becomes | $\vee$            |
| not                     | becomes | $\neg$            |
| it is not the case that | becomes | $\neg$            |
| if $p$ then $q$         | becomes | $p \Rightarrow q$ |

Page 33 of textbook

|         |         |          |
|---------|---------|----------|
| Means   | becomes | $\equiv$ |
| However | becomes | $\wedge$ |
| ;       | becomes | $\wedge$ |

# Modeling English propositions

---

**2.8** Translate the following English statement into a boolean expression.  $v$  is in  $b[1..10]$  means that if  $v$  is in  $b[11..20]$  then it is not in  $b[11..20]$ .

Let  $x$ : denote “ $v$  is in  $b[1 \cdots 10]$ ”

$y$ : denote “ $v$  is in  $b[11 \cdots 20]$ ”.

$$x \equiv y \Rightarrow \neg y$$

# Modeling English propositions

---

**2.10** Solve the following puzzle. A certain island is inhabited by people who either always tell the truth or always lie and who respond to questions with a yes or a no. A tourist comes to a fork in the road, where one branch leads to a restaurant and the other does not. There is no sign indicating which branch to take, but there is an islander standing at the fork. What single yes/no question can the tourist ask to find the way to the restaurant?

# Modeling English propositions

---

**2.10** Solve the following puzzle. A certain island is inhabited by people who either always tell the truth or always lie and who respond to questions with a yes or a no. A tourist comes to a fork in the road, where one branch leads to a restaurant and the other does not. There is no sign indicating which branch to take, but there is an islander standing at the fork. What single yes/no question can the tourist ask to find the way to the restaurant?

Hint: Let  $p$  stand for “the islander at the fork always tells the truth” and let  $q$  stand for “the left-hand branch leads to the restaurant”. Let  $E$  stand for a boolean expression such that, whether the islander tells the truth or lies, the answer to the question “Is  $E$  true?” will be yes iff the left-hand branch leads to the restaurant. Construct the truth table that  $E$  must have, in terms of  $p$  and  $q$ , and then design an appropriate  $E$  according to the truth table.

Hint:

Let

**$p$**  stands for islander at the fork always tell the **truth**

**$q$**  stands for “the left-hand branch leads to the restaurant

**$E$**  stand for a Boolean expression such that, whether the islander tells the truth or lies ,the answer to the question “Is  $E$  true?”

**Yes** iff the left-hand branch leads to the restaurant

Construct the truth table that  $E$  must have, in terms of  $p$  and  $q$  and then design an appropriate  $E$  according to the truth table.

**2.10** Solve the following puzzle. A certain island is inhabited by people who either always tell the truth or always lie and who respond to questions with a yes or a no. A tourist comes to a fork in the road, where one branch leads to a restaurant and the other does not. There is no sign indicating which branch to take, but there is an islander standing at the fork. What single yes/no question can the tourist ask to find the way to the restaurant?

- p*: The islander is truthful
- q*: Left Branch leads to the restaurant

| <i>p</i> | <i>q</i> | <i>E</i> |
|----------|----------|----------|
| T        | T        | T        |
| T        | F        | F        |
| F        | T        | F        |
| F        | F        | T        |

# Equivalence and true

---

(3.1) **Axiom, Associativity of  $\equiv$ :**  $((p \equiv q) \equiv r) \equiv (p \equiv (q \equiv r))$

Associativity allows us to be informal and insert or delete pairs of parentheses in sequences of equivalences, just as we do with sequences of additions (e.g.  $w + x + y + z$  is equivalent to  $w + (x + y) + z$ ). Hence, we can write

$p \equiv q \equiv r$  instead of  $p \equiv (q \equiv r)$  or  $(p \equiv q) \equiv r$  .

Keeping axiom (3.1) in mind, we express the second axiom, symmetry, without parentheses.

(3.2) **Axiom, Symmetry of  $\equiv$ :**  $p \equiv q \equiv q \equiv p$

You can see why this axiom is called *symmetry* by imagining parentheses as follows:  $(p \equiv q) \equiv (q \equiv p)$ .

We now give our first proof, of the following theorem:

$$p \equiv p \equiv q \equiv q \quad .$$

Remember that the axiom of associativity allows us to parenthesize an expression such as (3.2) in several ways. In the following proof, we parenthesize (3.2) as  $(p \equiv q \equiv q) \equiv p$ , so that, using Leibniz, we can replace  $p \equiv q \equiv q$  in an expression by  $p$ .

$$\begin{aligned} & p \equiv p \equiv q \equiv q \\ = & \quad \langle \text{Symmetry of } \equiv \text{ (3.2) —replace } p \equiv q \equiv q \text{ by } p \rangle \\ & p \equiv p \\ = & \quad \langle \text{Symmetry of } \equiv \text{ (3.2) —replace first } p \text{ by } p \equiv q \equiv q \rangle \\ & p \equiv q \equiv q \equiv p \end{aligned}$$



(3.3) **Axiom, Identity of  $\equiv$ :**  $true \equiv q \equiv q$

# Equivalence and true

---

## Two theorems

(3.4) *true*

(3.5) **Reflexivity of  $\equiv$ :**  $p \equiv p$

# Equivalence and true

---

## Two theorems

(3.4)  $true$

(3.5) **Reflexivity of  $\equiv$ :**  $p \equiv p$

(3.4)  $true$   
=  $\langle \text{Identity of } \equiv (3.3), \text{ with } q := true \rangle$   
 $true \equiv true$   
=  $\langle \text{Identity of } \equiv (3.3) \text{ —replace the second } true \rangle$   
 $true \equiv q \equiv q$  —Identity of  $\equiv (3.3)$

# Equivalence and true

---

## Two theorems

(3.4)  $true$

(3.5) **Reflexivity of  $\equiv$ :**  $p \equiv p$

(3.5)  $p \equiv p$

= < Use Identity (3.3) to replace the left  $p$  by  $(true \equiv p)$  >

$true \equiv p \equiv p$

# Negation, inequivalence, and false

---

(3.8) **Axiom, Definition of *false* :**  $false \equiv \neg true$

(3.9) **Axiom, Distributivity of  $\neg$  over  $\equiv$  :**  $\neg(p \equiv q) \equiv \neg p \equiv q$

(3.10) **Axiom, Definition of  $\neq$  :**  $(p \neq q) \equiv \neg(p \equiv q)$

# Negation, inequivalence, and false

## Theorems relating $\equiv$ , $\neq$ , $\neg$ , and *false*

$$(3.11) \quad \neg p \equiv q \equiv p \equiv \neg q$$

$$(3.12) \quad \text{Double negation: } \neg\neg p \equiv p$$

$$(3.13) \quad \text{Negation of false: } \neg\text{false} \equiv \text{true}$$

$$(3.14) \quad (p \neq q) \equiv \neg p \equiv q$$

$$(3.15) \quad \neg p \equiv p \equiv \text{false}$$

$$(3.16) \quad \text{Symmetry of } \neq: (p \neq q) \equiv (q \neq p)$$

$$(3.17) \quad \text{Associativity of } \neq: ((p \neq q) \neq r) \equiv (p \neq (q \neq r))$$

$$(3.18) \quad \text{Mutual associativity: } ((p \neq q) \equiv r) \equiv (p \neq (q \equiv r))$$

$$(3.19) \quad \text{Mutual interchangeability: } p \neq q \equiv r \equiv p \equiv q \neq r$$

# Negation, inequivalence, and false

(3.11) Proof  $\neg p \equiv q \equiv p \equiv \neg q$ :

$\neg p \equiv q$   
=<Use axiom (3.9)>  
 $\neg(p \equiv q)$   
=<Use axiom (3.2)>  
 $\neg(q \equiv p)$   
=<Use axiom (3.9)>  
 $\neg q \equiv p$   
=<Use axiom (3.2)>  
 $p \equiv \neg q$

(3.12) Proof  $\neg\neg p \equiv p$ :

$\neg\neg p$   
=<Use axiom (3.3)>  
 $\neg\neg(true \equiv p)$   
=<Use axiom (3.3) on true>  
 $\neg\neg(p \equiv p \equiv p)$   
=<Use axiom (3.9)>  
 $\neg(\neg p \equiv p \equiv p)$   
=<Use axiom (3.2)>  
 $\neg(p \equiv \neg p \equiv p)$   
=<Use axiom (3.9)>  
 $\neg p \equiv \neg p \equiv p$   
=<Use axiom (3.3)>  
 $true \equiv p$   
=<Use axiom (3.3)>  
 $p$

(3.13) Proof  $\neg false \equiv true$ :

$\neg false$   
=<Use axiom (3.8)>  
 $\neg\neg true$   
=<Use theorem (3.12)>  
 $true$

(3.14) Proof  $(p \neq q) \equiv \neg p \equiv q$ :

$(p \neq q)$   
=<Use axiom (3.10)>  
 $\neg(p \equiv q)$   
=<Use axiom (3.9)>  
 $\neg p \equiv q$

# Negation, inequivalence, and false

(3.15) Proof  $\neg p \equiv p \equiv \text{false}$ :

$\neg p \equiv p$   
 =<Use axiom (3.9)>  
 $\neg(p \equiv p)$   
 =<Use axiom (3.3)>  
 $\neg(\text{true})$   
 =<Use axiom (3.8)>  
 $\text{false}$

(3.16) Proof  $(p \not\equiv q) \equiv (q \not\equiv p)$ :

$(p \not\equiv q)$   
 =<Use axiom (3.10)>  
 $\neg(p \equiv q)$   
 =<Use axiom (3.2)>  
 $\neg(q \equiv p)$   
 =<Use axiom (3.10)>  
 $(q \not\equiv p)$

(3.17) Proof  $((p \not\equiv q) \not\equiv r) \equiv (p \not\equiv (q \not\equiv r))$ :

$((p \not\equiv q) \not\equiv r)$   
 =<Use theorem (3.14) and axiom (3.2)>  
 $((q \equiv \neg p) \not\equiv r)$   
 =<Use theorem (3.14)>  
 $(\neg(q \equiv \neg p) \equiv r)$   
 =<Use axiom (3.9)>  
 $(\neg q \equiv \neg p \equiv r)$   
 =<Use axiom (3.2) and axiom (3.1)>  
 $(\neg p \equiv (\neg q \equiv r))$   
 =<Use theorem (3.14)>  
 $(\neg p \equiv (q \not\equiv r))$   
 =<Use theorem (3.14)>  
 $(p \not\equiv (q \not\equiv r))$

(3.18) Proof  $((p \not\equiv q) \equiv r) \equiv (p \not\equiv (q \equiv r))$ :

$((p \not\equiv q) \equiv r)$   
 =<Use theorem (3.14) and axiom (3.1)>  
 $(\neg p \equiv (q \equiv r))$   
 =<Use theorem (3.14)>  
 $(p \not\equiv (q \equiv r))$



# Negation, inequivalence, and false

---

(3.19) Proof  $p \not\equiv q \equiv r \equiv p \equiv q \not\equiv r$ :

$$p \not\equiv q \equiv r$$

=<Use axiom (3.10)>

$$\neg(p \equiv q) \equiv r$$

=<Use axiom (3.2) then axiom (3.9)>

$$\neg q \equiv p \equiv r$$

=<Use axiom (3.2) then axiom (3.9)>

$$p \equiv \neg(q \equiv r)$$

=<Use axiom (3.10)>

$$p \equiv q \not\equiv r$$

# Disjunction

---

(3.24) **Axiom, Symmetry of  $\vee$ :**  $p \vee q \equiv q \vee p$

(3.25) **Axiom, Associativity of  $\vee$ :**  $(p \vee q) \vee r \equiv p \vee (q \vee r)$

(3.26) **Axiom, Idempotency<sup>7</sup> of  $\vee$ :**  $p \vee p \equiv p$

(3.27) **Axiom, Distributivity of  $\vee$  over  $\equiv$ :**

$$p \vee (q \equiv r) \equiv p \vee q \equiv p \vee r$$

(3.28) **Axiom, Excluded Middle:**  $p \vee \neg p$

# Disjunction

---

## Theorems concerning $\vee$

(3.29) **Zero**<sup>8</sup> of  $\vee$ :  $p \vee \text{true} \equiv \text{true}$

(3.30) **Identity** of  $\vee$ :  $p \vee \text{false} \equiv p$

(3.31) **Distributivity** of  $\vee$  over  $\wedge$ :  $p \vee (q \wedge r) \equiv (p \vee q) \wedge (p \vee r)$

(3.32)  $p \vee q \equiv p \vee \neg q \equiv p$

# Disjunction

---

(3.29) Proof  $p \vee \text{true} \equiv \text{true}$ :

$p \vee \text{true}$   
= $\langle$ Use axiom (3.3) $\rangle$   
 $p \vee (p \equiv p)$   
= $\langle$ Use axiom (3.27) $\rangle$   
 $p \vee p \equiv p \vee p$   
= $\langle$ Use axiom (3.26) $\rangle$   
 $p \equiv p$   
= $\langle$ Use axiom (3.3) $\rangle$   
 $\text{true}$

(3.30) Proof  $p \vee \text{false} \equiv p$ :

$p \vee \text{false}$   
= $\langle$ Use axiom (3.8) and axiom (3.3) $\rangle$   
 $p \vee \neg(p \equiv p)$   
= $\langle$ Use axiom (3.9) $\rangle$   
 $p \vee (\neg p \equiv p)$   
= $\langle$ Use axiom (3.27) $\rangle$   
 $p \vee \neg p \equiv p \vee p$   
= $\langle$ Use axiom (3.28) and axiom (3.26) $\rangle$   
 $\text{true} \equiv p$   
= $\langle$ Use axiom (3.3) $\rangle$   
 $p$

# Disjunction

---

Prove Distributivity of  $\vee$  over  $\wedge$  (3.31),  $p \vee (q \wedge r) \equiv (p \vee q) \wedge (p \vee r)$ .

The proof requires only the symmetry, associativity, and idempotency of  $\vee$ .

Proof of Distributivity of  $\vee$  over  $\wedge$ , (3.31),  $p \vee (q \wedge r) \equiv (p \vee q) \wedge (p \vee r)$ .

|  |  |
|--|--|
| $(p \vee q) \vee (p \vee r)$                                     |  |
| $= \langle \text{Associativity of } \vee \text{ (3.25)} \rangle$ | <b>(3.25) Axiom, Associativity of <math>\vee</math>: <math>(p \vee q) \vee r \equiv p \vee (q \vee r)</math></b> |
| $p \vee (q \vee p) \vee r$                                       |  |
| $= \langle \text{Symmetry of } \vee \text{ (3.24)} \rangle$      | <b>(3.24) Axiom, Symmetry of <math>\vee</math>: <math>p \vee q \equiv q \vee p</math></b>                        |
| $p \vee (p \vee q) \vee r$                                       |  |
| $= \langle \text{Associativity of } \vee \text{ (3.25)} \rangle$ | <b>(3.25) Axiom, Associativity of <math>\vee</math>: <math>(p \vee q) \vee r \equiv p \vee (q \vee r)</math></b> |
| $(p \vee p) \vee (q \vee r)$                                     |  |
| $= \langle \text{Idempotency of } \vee \text{ (3.26)} \rangle$   | <b>(3.26) Axiom, Idempotency of <math>\vee</math>: <math>p \vee p \equiv p</math></b>                            |
| $p \vee (q \vee r)$  |  |

# Disjunction

---

(3.32) Proof  $p \vee q \equiv p \vee \neg q \equiv p$ :

$$p \vee q \equiv p \vee \neg q$$

=<Use axiom (3.27)>

$$p \vee (q \equiv \neg q)$$

=<Use axiom (3.2) and axiom (3.9)>

$$p \vee \neg(q \equiv q)$$

=<Use axiom (3.3)>

$$p \vee \neg(true)$$

=<Use axiom (3.8)>

$$p \vee false$$

=<Use theorem (3.30)>

$$p$$

# Conjunction

---

(3.35) **Axiom, Golden rule** :  $p \wedge q \equiv p \equiv q \equiv p \vee q$

# Conjunction

---

## Basic properties of $\wedge$

(3.36) **Symmetry of  $\wedge$ :**  $p \wedge q \equiv q \wedge p$

(3.37) **Associativity of  $\wedge$ :**  $(p \wedge q) \wedge r \equiv p \wedge (q \wedge r)$

(3.38) **Idempotency of  $\wedge$ :**  $p \wedge p \equiv p$

(3.39) **Identity of  $\wedge$ :**  $p \wedge \text{true} \equiv p$

(3.40) **Zero of  $\wedge$ :**  $p \wedge \text{false} \equiv \text{false}$

(3.41) **Distributivity of  $\wedge$  over  $\vee$ :**

$$p \wedge (q \vee r) \equiv (p \wedge q) \vee (p \wedge r)$$

(3.42) **Contradiction:**  $p \wedge \neg p \equiv \text{false}$



# Conjunction

---

## Theorems relating $\wedge$ and $\vee$

(3.43) **Absorption:** (a)  $p \wedge (p \vee q) \equiv p$

(b)  $p \vee (p \wedge q) \equiv p$

(3.44) **Absorption:** (a)  $p \wedge (\neg p \vee q) \equiv p \wedge q$

(b)  $p \vee (\neg p \wedge q) \equiv p \vee q$

(3.45) **Distributivity of  $\vee$  over  $\wedge$ :**

$$p \vee (q \wedge r) \equiv (p \vee q) \wedge (p \vee r)$$

(3.46) **Distributivity of  $\wedge$  over  $\vee$ :**

$$p \wedge (q \vee r) \equiv (p \wedge q) \vee (p \wedge r)$$

(3.47) **De Morgan:** (a)  $\neg(p \wedge q) \equiv \neg p \vee \neg q$

(b)  $\neg(p \vee q) \equiv \neg p \wedge \neg q$

# Conjunction

(3.36) Proof  $p \wedge q \equiv q \wedge p$ :

$$\begin{aligned}
 & p \wedge q \\
 = & \langle \text{Use axiom (3.35)} \rangle \\
 & p \equiv q \equiv p \vee q \\
 = & \langle \text{Use axiom (3.2) and axiom (3.24)} \rangle \\
 & q \equiv p \equiv q \vee p \\
 = & \langle \text{Use axiom (3.35)} \rangle \\
 & q \wedge p
 \end{aligned}$$

(3.37)  $(p \wedge q) \wedge r \equiv p \wedge (q \wedge r)$

$$\begin{aligned}
 & (p \wedge q) \wedge r \\
 = & \langle \text{Golden rule (3.35)} \rangle \\
 & (p \equiv q \equiv p \vee q) \wedge r \\
 = & \langle \text{Golden rule (3.35), with } p, q := (p \equiv q \equiv p \vee q), r \rangle \\
 & p \equiv q \equiv p \vee q \equiv r \equiv (p \equiv q \equiv p \vee q) \vee r \\
 = & \langle \text{Distributivity of } \vee \text{ over } \equiv \text{ (3.27)} \rangle \\
 & p \equiv q \equiv p \vee q \equiv r \equiv p \vee r \equiv q \vee r \equiv p \vee q \vee r \\
 = & \langle \text{Symmetry and associativity of } \equiv \text{ and } \vee \rangle \\
 & p \equiv q \equiv r \equiv p \vee q \equiv q \vee r \equiv r \vee p \equiv p \vee q \vee r
 \end{aligned}$$

(3.55)  $(p \wedge q) \wedge r \equiv$

$$\begin{aligned}
 & p \equiv q \equiv r \equiv p \vee q \equiv q \vee r \equiv r \vee p \equiv p \vee q \vee r \\
 & p \wedge (q \wedge r) \\
 = & \langle \text{Symmetry of } \wedge \text{ (3.36)} \rangle \\
 & (q \wedge r) \wedge p \\
 = & \langle (3.55), \text{ with } p, q, r := q, r, p \rangle \\
 & q \equiv r \equiv p \equiv q \vee r \equiv r \vee p \equiv p \vee q \equiv q \vee r \vee p \\
 = & \langle \text{Symmetry and associativity of } \equiv \text{ and } \vee \rangle \\
 & p \equiv q \equiv r \equiv p \vee q \equiv q \vee r \equiv r \vee p \equiv p \vee q \vee r \\
 = & \langle (3.55) \rangle \\
 & (p \wedge q) \wedge r
 \end{aligned}$$

# Conjunction

---

Use the Golden rule (3.35) for every expression containing a conjunction. (3.38) to (3.42) are all similar to disjunction proofs after the Golden rule is applied.

(3.43)(a) Proof  $p \wedge (p \vee q) \equiv p$ :

$$p \wedge (p \vee q)$$

=<Use axiom (3.35)>

$$p \equiv (p \vee q) \equiv p \vee (p \vee q)$$

=<Use axiom (3.25) and axiom (3.26)>

$$p \equiv p \vee q \equiv p \vee q$$

=<Use axiom (3.2)>

$$p \equiv \text{true}$$

=<Use axiom (3.2)>

$$p$$

(3.44)(a) Proof  $p \wedge (\neg p \vee q) \equiv p \wedge q$ :

$$p \wedge (\neg p \vee q)$$

=<Use axiom (3.35)>

$$p \equiv (\neg p \vee q) \equiv p \vee (\neg p \vee q)$$

=<Use axiom (3.25), axiom (3.28)>

$$p \equiv (\neg p \vee q) \equiv \text{true} \vee q$$

=<Use theorem (3.29) and axiom (3.3)>

$$p \equiv (\neg p \vee q)$$

=<Use theorem (3.32) with  $p,q:=q,p$ >

$$p \equiv (p \vee q) \equiv q$$

=<Use axiom (3.2) and axiom (3.35)>

$$p \wedge q$$

# Conjunction

Use the Golden rule (3.35) for every expression containing a conjunction. (3.38) to (3.42) are all similar to disjunction proofs after the Golden rule is applied.

(3.45) Proof  $p \vee (q \wedge r) \equiv (p \vee q) \wedge (p \vee r)$ :

$$\begin{aligned}
 & p \vee (q \wedge r) \\
 = & \text{<Use axiom (3.35)>} \\
 & p \vee (q \equiv r \equiv q \vee r) \\
 = & \text{<Use axiom (3.27)>} \\
 & p \vee q \equiv p \vee r \equiv p \vee (q \vee r) \\
 = & \text{<Use theorem (3.31)>} \\
 & p \vee q \equiv p \vee r \equiv (p \vee q) \vee (p \vee r) \\
 = & \text{<Use axiom (3.35)>} \\
 & (p \vee q) \wedge (p \vee r)
 \end{aligned}$$

(3.46) Proof  $p \wedge (q \vee r) \equiv (p \wedge q) \vee (p \wedge r)$ :

$$\begin{aligned}
 & (p \wedge q) \vee (p \wedge r) \\
 = & \text{<Use axiom (3.35)>} \\
 & (p \equiv q \equiv p \vee q) \vee (p \equiv r \equiv p \vee r) \\
 = & \text{<Use axiom (3.27)>} \\
 & (p \equiv q \equiv p \vee q) \vee p \equiv (p \equiv q \equiv p \vee q) \vee r \equiv (p \equiv q \equiv p \vee q) \vee (p \vee r) \\
 = & \text{<Use axiom (3.27) and axiom (3.25)>} \\
 & p \vee p \equiv q \vee p \equiv p \vee q \vee p \equiv p \vee r \equiv q \vee r \equiv p \vee q \vee r \equiv p \vee p \vee r \equiv q \vee p \vee r \equiv p \vee q \vee p \vee r \\
 = & \text{<Use axiom (3.26), axiom (3.24) and axiom (3.2)>} \\
 & p \equiv p \vee q \equiv p \vee q \equiv p \vee r \equiv q \vee r \equiv p \vee q \vee r \equiv p \vee r \equiv p \vee q \vee r \equiv p \vee q \vee r \\
 = & \text{<Use axiom (3.2) and axiom (3.3)>} \\
 & p \equiv \text{true} \equiv q \vee r \equiv p \vee q \vee r \equiv p \vee r \equiv p \vee r \equiv \text{true} \\
 = & \text{<Use axiom (3.2) and axiom (3.3)>} \\
 & p \equiv q \vee r \equiv p \vee q \vee r \equiv \text{true} \equiv \text{true} \equiv \text{true} \\
 = & \text{<Use axiom (3.3)>} \\
 & p \equiv q \vee r \equiv p \vee q \vee r \\
 = & \text{<Use axiom (3.25)>} \\
 & p \equiv q \vee r \equiv p \vee (q \vee r) \\
 = & \text{<Use axiom (3.35)>} \\
 & p \wedge (q \vee r)
 \end{aligned}$$

# Conjunction

---

(3.47)(a) Proof  $\neg(p \wedge q) \equiv \neg p \vee \neg q$ :

$$\neg(p \wedge q)$$

=<Use axiom (3.35)>

$$\neg(p \equiv q \equiv p \vee q)$$

=<Use axiom (3.9)>

$$\neg p \equiv q \equiv p \vee q$$

=<Use theorem (3.32) with  $p, q := q, p$  >

$$\neg p \equiv \neg p \vee q$$

=<Use theorem (3.32) with  $p, q := \neg p, q$  >

$$\neg p \vee \neg q$$

(3.48) Proof  $p \wedge q \equiv p \wedge \neg q \equiv \neg p$ :

$$p \wedge q \equiv p \wedge \neg q$$

=<Use theorem (3.12)>

$$\neg\neg(p \wedge q \equiv p \wedge \neg q)$$

=<Use axiom (3.9) with  $p, q := p \wedge q, p \wedge \neg q$  >

$$\neg(\neg(p \wedge q) \equiv p \wedge \neg q)$$

=<Use axiom (3.2) and axiom (3.9) with  $p, q := p \wedge \neg q, \neg(p \wedge q)$  >

$$\neg(p \wedge q) \equiv \neg(p \wedge \neg q)$$

=<Use axiom (3.2) and axiom (3.9) with  $p, q := p \wedge \neg q, \neg(p \wedge q)$  >

$$\neg(p \wedge q) \equiv \neg(p \wedge \neg q)$$

=<Use theorem (3.47)(a) >

$$\neg p \vee \neg q \equiv \neg p \vee q$$

=<Use theorem (3.32) with  $p, q := \neg p, q$  >

$$\neg p$$

# Conjunction

---

(3.49) Proof  $p \wedge (q \equiv r) \equiv p \wedge q \equiv p \wedge r \equiv p$ :

$$\begin{aligned}
 & p \wedge (q \equiv r) \\
 = & \langle \text{Use theorem (3.12)} \rangle \\
 & \neg \neg (p \wedge (q \equiv r)) \\
 = & \langle \text{Use theorem (3.47)(a)} \rangle \\
 & \neg (\neg p \vee \neg (q \equiv r)) \\
 = & \langle \text{Use axiom (3.9)} \rangle \\
 & \neg (\neg p \vee (\neg q \equiv r)) \\
 = & \langle \text{Use axiom (3.27)} \rangle \\
 & \neg (\neg p \vee \neg q \equiv \neg p \vee r) \\
 = & \langle \text{Use axiom (3.9) and theorem (3.47)(a)} \rangle \\
 & p \wedge q \equiv \neg p \vee r \\
 = & \langle \text{Use theorem (3.32) with } p, q := r, p \rangle \\
 & p \wedge q \equiv p \vee r \equiv r \\
 = & \langle \text{Use axiom (3.3) twice} \rangle \\
 & p \wedge q \equiv p \vee r \equiv r \equiv p \equiv p \\
 = & \langle \text{Use axiom (3.35)} \rangle \\
 & p \wedge q \equiv p \wedge r \equiv p
 \end{aligned}$$

(3.50) Proof  $p \wedge (q \equiv p) \equiv p \wedge q$ :

$$\begin{aligned}
 & p \wedge (q \equiv p) \\
 = & \langle \text{Use theorem (3.49) with } p, q, r := p, q, p \rangle \\
 & p \wedge q \equiv p \wedge p \equiv p \\
 = & \langle \text{Use theorem (3.38)} \rangle \\
 & p \wedge q \equiv \text{true} \\
 = & \langle \text{Use axiom (3.3)} \rangle \\
 & p \wedge q
 \end{aligned}$$

(3.51) Proof  $(p \equiv q) \wedge (r \equiv p) \equiv (p \equiv q) \wedge (r \equiv q)$ :

$$\begin{aligned}
 & (p \equiv q) \wedge (r \equiv p) \\
 = & \langle \text{Use theorem (3.49) with } p, q, r := (r \equiv p), p, q \rangle \\
 & (r \equiv p) \wedge p \equiv (r \equiv p) \wedge q \equiv (r \equiv p) \\
 = & \langle \text{Use theorem (3.50)} \rangle \\
 & p \wedge r \equiv (r \equiv p) \wedge q \equiv r \equiv p \\
 = & \langle \text{Use theorem (3.49)} \rangle \\
 & p \wedge r \equiv r \wedge q \equiv p \wedge q \equiv q \equiv r \equiv p \\
 = & \langle \text{Use theorem (3.50)} \rangle \\
 & p \wedge r \equiv q \wedge (r \equiv q) \equiv p \wedge q \equiv q \equiv r \equiv p \\
 = & \langle \text{Use theorem (3.49)} \rangle \\
 & p \wedge (r \equiv q) \equiv q \wedge (r \equiv q) \equiv q \equiv r \\
 = & \langle \text{Use theorem (3.49) and symmetry of } \equiv \text{ and } \wedge \rangle \\
 & (p \equiv q) \wedge (r \equiv p) \equiv (p \equiv q) \wedge (r \equiv q)
 \end{aligned}$$

# Any Questions?

---